@prefix rdfs:   <http://www.w3.org/2000/01/rdf-schema#>.
@prefix owl:    <http://www.w3.org/2002/07/owl#>.
@prefix xsd:    <http://www.w3.org/2001/XMLSchema#> .

@prefix dct:    <http://purl.org/dc/terms/>.
@prefix fabio:  <http://purl.org/spar/fabio/> .
@prefix frbr:   <http://purl.org/vocab/frbr/core#>.
@prefix oa:     <http://www.w3.org/ns/oa#>.

@prefix issa:   <http://data-issa.instance.fr/>.
@prefix issap:  <http://data-issa.instance.fr/property/>.


# -- Document metadata custom classes and properties ---
issa:DocumentBody
    a                       owl:Class;
    owl:equivalentClass     <http://ns.inria.fr/covid19/DocumentBody>;
    rdfs:subClassOf         fabio:Work;
    rdfs:label              "document body";
    dct:description         "A work's body, e.g. the main part of a research article";
    .

issap:hasTitle
    a                       owl:ObjectProperty;
    owl:equivalentProperty  <http://ns.inria.fr/covid19/property/hasTitle>;
    rdfs:subPropertyOf      frbr:part;
    rdfs:label              "has title";
    dct:description         "Links a work to its title";
    .

issap:hasAbstract
    a                       owl:ObjectProperty;
    rdfs:subPropertyOf      frbr:part;
    rdfs:label              "has abstract";
    dct:description         "Links a work to its abstract";
    owl:sameAs              dct:abstract;
    owl:equivalentProperty  dct:abstract;
    .

issap:hasBody
    a                       owl:ObjectProperty;
    rdfs:subPropertyOf      frbr:part;
    owl:equivalentProperty  <http://ns.inria.fr/covid19/property/hasBody>;
    rdfs:label              "has body";
    dct:description         "Links a work to its body, e.g. the main part of a research article";
    .

issap:institutionList
    a                       owl:ObjectProperty;
    rdfs:label              "has institutions";
    dct:description         "Links an author to the institutions/organizations he/she is affiliated to (ordered list). It complements foaf:member that links to organizations without order.";
    .


# --- Annotations classes and properties ---

issap:confidence
    a                       owl:DatatypeProperty;
    owl:equivalentProperty  <http://ns.inria.fr/covid19/property/confidence>;
    rdfs:label              "entity confidence score";
    dct:description         "Confidence score obtained during the named entity recognition process";
    .

issap:rank
    a                       owl:DatatypeProperty;
    rdfs:label              "entity's indexing rank";
    dct:description         "Indexing rank is a place of a descriptor in the list of descriptors ordered by descending confidence score";
    .

# The body of this annotation would be a URI of a thematic vocabulary; for example, an Agrovoc concept.
issa:ThematicDesciptorAnnotation
    a                       owl:Class;
    rdfs:subClassOf         oa:Annotation;
    rdfs:label              "thematic descriptor";
    dct:description         "Document's non-geographical thematic descriptor";
    .

# The body of this annotation would be a URI of a geographical vocabulary; for example, an Agrovoc concept or a GeoName concept.
issa:GeographicDescriptorAnnotation
    a                       owl:Class;
    rdfs:subClassOf         oa:Annotation;
    rdfs:label              "geographical annotation";
    dct:description         "Document's geographical descriptor";
    .

# The body of this annotation would be a URI of a domain vocabulary; for example, an AGRIS concept.
issa:DomainAnnotation
    a                       owl:Class;
    rdfs:subClassOf         oa:Annotation;
    rdfs:label              "domain annotation";
    dct:description         "Document's domain/discipline (branch of knowledge)";
    .

# The body of this annotation would be a blank node [ a oa:TextualBody ; rdf:value "keyword"; dc:language "en" ; dc:format "text"].
issa:AuthorKeywordAnnotation
    a                       owl:Class;
    rdfs:subClassOf         oa:Annotation;
    rdfs:label              "author keyword annotation";
    dct:description         "Document's author keyword descriptor";
    .


# The body of this annotation would be the URI of an SDG in the form https://metadata.un.org/sdg/xx
issa:OpenAlexSdgAnnotation
    a                       owl:Class;
    rdfs:subClassOf         oa:Annotation;
    rdfs:label              "OpenAlex's Sustainable Development Goal annotation";
    dct:description         "Document's Sustainable Development Goal according to OpenAlex classification";
    .

# The body of this annotation would be the URI of an OpenAlex domain https://docs.openalex.org/api-entities/topics/topic-object#domain
issa:OpenAlexDomainAnnotation
    a                       owl:Class;
    rdfs:subClassOf         oa:Annotation;
    rdfs:label              "OpenAlex's domain annotation";
    dct:description         "Document's domain according to OpenAlex topics/subfield/field/domain classification";
    .

# The body of this annotation would be the URI of an OpenAlex field https://docs.openalex.org/api-entities/topics/topic-object#field
issa:OpenAlexFieldAnnotation
    a                       owl:Class;
    rdfs:subClassOf         oa:Annotation;
    rdfs:label              "OpenAlex's field annotation";
    dct:description         "Document's field according to OpenAlex topics/subfield/field/domain classification";
    .

# The body of this annotation would be the URI of an OpenAlex subfield https://docs.openalex.org/api-entities/topics/topic-object#subfield
issa:OpenAlexSubfieldAnnotation
    a                       owl:Class;
    rdfs:subClassOf         oa:Annotation;
    rdfs:label              "OpenAlex's subfield annotation";
    dct:description         "Document's subfield according to OpenAlex topics/subfield/field/domain classification";
    .

# The body of this annotation would be the URI of an OpenAlex topic https://docs.openalex.org/api-entities/topics/topic-object#id
issa:OpenAlexTopicAnnotation
    a                       owl:Class;
    rdfs:subClassOf         oa:Annotation;
    rdfs:label              "OpenAlex's topic annotation";
    dct:description         "Document's topic according to OpenAlex topics/subfield/field/domain classification";
    .
